Q2 (complete)

ex2/lists.v
@@ -1,18 +1,25 @@
 Set Implicit Arguments.
 Require Import Lists.List.
 Import ListNotations.
+Require Import List.
+Require Import Arith.
 Require Import Lia.
+Import Nat.
 
 Print list.
 Print rev.
 
 
-(* Q1. Define `is_sorted`.  (should return a Prop.)  *)
+
+(* Q1. Define is_sorted.  (returns a Prop.)  *)  
+
 Inductive is_sorted {A : Type} (R : A -> A -> Prop) : list A -> Prop :=
 | sorted_nil : is_sorted R []
 | sorted_singleton : forall x, is_sorted R [x]
-| sorted_cons : forall x y l, R x y -> is_sorted R (y :: l) -> is_sorted R (x :: y :: l).
-
+| sorted_cons : forall x y l, 
+  R x y -> 
+  is_sorted R (y :: l) -> 
+  is_sorted R (x :: y :: l).
 
 (* Show that this list is sorted. *)
 Lemma warm_up : is_sorted le [3;5;9].
@@ -22,39 +29,46 @@ Proof.
   apply sorted_singleton.
 Qed.
 
-
 (* Q2. Prove that an ascending list of nat, when reversed, 
  *     becomes a descending list. *)
-Lemma sorted_append_one :
-  forall (A : Type) (R : A -> A -> Prop) (l : list A) (a b : A),
-    is_sorted R (l ++ [a]) ->
-    R a b ->
-    is_sorted R (l ++ [a; b]).
+
+Lemma aux_rev_lemma : forall (A : Set) (l : list A) R a b,
+                        is_sorted R (l ++ [a]) -> R a b -> 
+                        is_sorted R (l ++ [a;b]).
 Proof.
-  intros A R l a b Hsorted Rab.
-  induction l as [| x xs IH].
+  intros.
+  (* intros A R l a b Hsorted Rab. *)
+  induction l as [| x xTail IH].
   - simpl in *. (* [] ++ [a] = [a], so goal becomes is_sorted R [a; b] *)
-    apply sorted_cons. assumption. apply sorted_singleton.
-  - simpl in *. (* l = x :: xs, so l ++ [a] = x :: xs ++ [a] *)
-    destruct xs as [| y ys].
-    + inversion Hsorted as [| | x' y' l' Hxy Hsorted']; subst.
-      apply sorted_cons. assumption.
-      apply sorted_cons. assumption. constructor.
-    + inversion Hsorted as [| | x' y' l' Hxy Hsorted']; subst.
-      apply sorted_cons. assumption.
-      apply IH. assumption.
+    apply sorted_cons. 
+    + assumption. 
+    + apply sorted_singleton.
+  - simpl in *. (* l = x :: xTail, so l ++ [a] = x :: xTail ++ [a] *)
+    destruct xTail as [| y yTail].
+    + inversion H; subst.
+      apply sorted_cons. 
+      * assumption.
+      * apply sorted_cons. 
+        -- assumption. 
+        -- apply sorted_singleton.
+    + inversion H; subst.
+      apply sorted_cons. 
+      * assumption.
+      * apply IH. assumption.
 Qed.
 
 (*     Don't forget to use the _hint_ when proving it. *)
 
-Theorem rev_asc_desc :
-  forall l, is_sorted le l -> is_sorted ge (rev l).
+Theorem rev_asc_desc :  forall l, 
+                        is_sorted le l -> is_sorted ge (rev l).
 Proof.
   intros l H.
   induction H.
   - simpl. constructor.
   - simpl. constructor.
-  - simpl.
+  - simpl in *.
     rewrite <- app_assoc.
-    apply (sorted_append_one nat ge rev l ++ [y; x]); auto. (* Does not work yet *)
+    apply aux_rev_lemma. 
+    + assumption.
+    + assumption.
 Qed.
